Added substitution maplet deletion and almost complete HRD composition proof

utp/utp_expr.thy
@@ -252,9 +252,10 @@ consts
   ucard   :: "'f \<Rightarrow> nat"
 
 definition "LNil = Nil"
+definition "LZero = 0"
 
 adhoc_overloading
-  uempty 0 and uempty LNil and
+  uempty LZero and uempty LNil and
   uapply fun_apply and uapply nth and uapply pfun_app and uapply ffun_app and
   uupd pfun_upd and uupd ffun_upd and uupd list_update and
   udom Domain and udom pdom and udom fdom and udom seq_dom and
@@ -431,6 +432,7 @@ lemmas uexpr_defs =
   ulim_right_def
   ucont_on_def
   LNil_def
+  LZero_def
 
 subsection {* Evaluation laws for expressions *}
 
